@prefix schema: <http://schema.org/> .
@prefix bibo: <http://purl.org/ontology/bibo/> .
@prefix dc: <http://purl.org/dc/elements/1.1/> .
@prefix dcat: <http://www.w3.org/ns/dcat#> .
@prefix dct: <http://purl.org/dc/terms/> .
@prefix dcterms: <http://purl.org/dc/terms/> .
@prefix dctype: <http://purl.org/dc/dcmitype/> .
@prefix eli: <http://data.europa.eu/eli/ontology#> .
@prefix foaf: <http://xmlns.com/foaf/0.1/> .
@prefix owl: <http://www.w3.org/2002/07/owl#> .
@prefix rdf: <http://www.w3.org/1999/02/22-rdf-syntax-ns#> .
@prefix rdfa: <http://www.w3.org/ns/rdfa#> .
@prefix rdfs: <http://www.w3.org/2000/01/rdf-schema#> .
@prefix schema: <http://schema.org/> .
@prefix skos: <http://www.w3.org/2004/02/skos/core#> .
@prefix snomed: <http://purl.bioontology.org/ontology/SNOMEDCT/> .
@prefix void: <http://rdfs.org/ns/void#> .
@prefix xml: <http://www.w3.org/XML/1998/namespace> .
@prefix xsd: <http://www.w3.org/2001/XMLSchema#> .
@prefix xsd1: <hhttp://www.w3.org/2001/XMLSchema#> .

@prefix geoschemas: <http://geoschemas.org/> .


geoschemas:FieldSite a rdfs:Class ;
    rdfs:label "FieldSite" ;
    rdfs:comment "A field site is a research site where where people conduct field research activities. Field research, field studies, or fieldwork is the collection of raw data outside a laboratory, library, or workplace setting." ;
    rdfs:subClassOf geoschemas:ResearchSite .


schema:GeoCircle a rdfs:Class ;
    rdfs:label "GeoCircle" ;
    rdfs:comment """A GeoCircle is a GeoShape representing a circular geographic area. As it is a GeoShape
          it provides the simple textual property 'circle', but also allows the combination of postalCode alongside geoRadius.
          The center of the circle can be indicated via the 'geoMidpoint' property, or more approximately using 'address', 'postalCode'.""" ;
    rdfs:subClassOf schema:GeoShape .

schema:GeoCoordinates a rdfs:Class ;
    rdfs:label "GeoCoordinates" ;
    rdfs:comment "The geographic coordinates of a place or event." ;
    rdfs:subClassOf schema:StructuredValue .

schema:GeoShape a rdfs:Class ;
    rdfs:label "GeoShape" ;
    dct:source <http://www.w3.org/wiki/WebSchemas/SchemaDotOrgSources#source_rNews> ;
    rdfs:comment "The geographic shape of a place. A GeoShape can be described using several properties whose values are based on latitude/longitude pairs. Either whitespace or commas can be used to separate latitude and longitude; whitespace should be used when writing a list of several such points." ;
    rdfs:subClassOf schema:StructuredValue .

schema:Place a rdfs:Class ;
    rdfs:label "Place" ;
    rdfs:comment "Entities that have a somewhat fixed, physical extension." ;
    rdfs:subClassOf schema:Thing .

geoschemas:ResearchActivity a rdfs:Class ;
    rdfs:label "ResearchActivity" ;
    rdfs:comment "A scientific research activity is something that occurs over a period of time and acts upon or with research entities; it may include consuming, processing, transforming, modifying, relocating, using, or generating entities." ;
    rdfs:subClassOf prov:Activity .

geoschemas:ResearchSite a rdfs:Class ;
    rdfs:label "ResearchSite" ;
    rdfs:comment "A research site is a place where people conduct research activities. Common research sites include universities, hospitals, research institutes, and field research locations." ;
    schema:sameAs <http://www.wikidata.org/entity/Q57951700> ;
    rdfs:subClassOf schema:Place .

schema:Thing a rdfs:Class ;
    rdfs:label "Thing" ;
    rdfs:comment "The most generic type of item." .
